specs/lemmas/Spec.Blake2.Lemmas.fst
@@ -8,112 +8,104 @@ open FStar.Mul
 
 friend Spec.Agile.Hash
 
+// AF: These proofs were extremely brittle when trying to do them directly on add_extra_i
+// The workaround here is overly verbose, but seems to add stability
 
 #push-options "--fuel 0 --ifuel 0"
 
 noextract inline_for_extraction
 let add_extra_i (a:hash_alg{is_blake a}) (ev:extra_state a) (i:U32.t) : extra_state a =
-  match a with
-  | Blake2S ->
     [@inline_let] let s = to_u64 i *. u64 (size_block a) in
     ev +. s
-  | Blake2B -> admit()
-    // [@inline_let] let s = to_u128 i *. u128 (size_block a) in
-    // ev +. s
 
 let add_extra_s (a:hash_alg{is_blake a}) (ev:nat) (i:nat) : nat =
-  match a with
-  | Blake2S -> (ev + (i * size_block a)) % pow2 64
-  | Blake2B -> admit()
+  (ev + (i * size_block a)) % pow2 64
 
-let add_s_i_2s (ev:extra_state Blake2S) (i:U32.t) : Lemma
-  (v (add_extra_i Blake2S ev i) == add_extra_s Blake2S (v ev) (v i))
+let add_s_i (a:hash_alg{is_blake a}) (ev:extra_state a) (i:U32.t) : Lemma
+  (v #U64 #SEC (add_extra_i a ev i) == add_extra_s a (v #U64 #SEC ev) (v i))
   = calc (==) {
-      v (add_extra_i Blake2S ev i);
+      v #U64 #SEC (add_extra_i a ev i);
       (==) { }
-      v (ev +. (to_u64 i *. u64 (size_block Blake2S)));
+      v (ev +. (to_u64 i *. u64 (size_block a)));
       (==) { }
-      (v ev + (v i * size_block Blake2S) % pow2 64) % pow2 64;
-      (==) { FStar.Math.Lemmas.lemma_mod_add_distr (v ev) (v i * size_block Blake2S) (pow2 64) }
-      (v ev + v i * size_block Blake2S) % pow2 64;
+      (v #U64 #SEC ev + (v i * size_block a) % pow2 64) % pow2 64;
+      (==) { FStar.Math.Lemmas.lemma_mod_add_distr (v #U64 #SEC ev) (v i * size_block a) (pow2 64) }
+      (v #U64 #SEC ev + v i * size_block a) % pow2 64;
     }
 
-let add_extra_s_zero_2s (ev:extra_state Blake2S) : Lemma (add_extra_s Blake2S (v ev) 0 == v ev)
+let add_extra_s_zero (#a:hash_alg{is_blake a}) (ev:extra_state a) : Lemma (add_extra_s a (v #U64 #SEC ev) 0 == v #U64 #SEC ev)
   = ()
 
-let add_extra_i_zero a ev = match a with
-  | Blake2S ->
-    add_s_i_2s ev 0ul;
-    add_extra_s_zero_2s ev
+let add_extra_i_zero a ev =
+    add_s_i a ev 0ul;
+    add_extra_s_zero ev
 
-  | Blake2B -> admit()
-
-let add_extra_s_assoc_2s (ev:nat) (i j:nat) : Lemma
-  (add_extra_s Blake2S (add_extra_s Blake2S ev j) i == add_extra_s Blake2S ev (i + j))
+let add_extra_s_assoc (a:hash_alg{is_blake a}) (ev:nat) (i j:nat) : Lemma
+  (add_extra_s a (add_extra_s a ev j) i == add_extra_s a ev (i + j))
   = calc (==) {
-      add_extra_s Blake2S (add_extra_s Blake2S ev j) i;
+      add_extra_s a (add_extra_s a ev j) i;
       (==) { }
-      ((add_extra_s Blake2S ev j) + (i * size_block Blake2S)) % pow2 64;
+      ((add_extra_s a ev j) + (i * size_block a)) % pow2 64;
       (==) { }
-      ((ev + (j * size_block Blake2S)) % pow2 64 + (i * size_block Blake2S)) % pow2 64;
-      (==) { FStar.Math.Lemmas.lemma_mod_add_distr (i * size_block Blake2S)
-        (ev + (j * size_block Blake2S)) (pow2 64) }
-      (ev + i * size_block Blake2S + j * size_block Blake2S) % pow2 64;
-      (==) { FStar.Math.Lemmas.distributivity_add_left i j (size_block Blake2S) }
-      add_extra_s Blake2S ev (i+j);
+      ((ev + (j * size_block a)) % pow2 64 + (i * size_block a)) % pow2 64;
+      (==) { FStar.Math.Lemmas.lemma_mod_add_distr (i * size_block a)
+        (ev + (j * size_block a)) (pow2 64) }
+      (ev + i * size_block a + j * size_block a) % pow2 64;
+      (==) { FStar.Math.Lemmas.distributivity_add_left i j (size_block a) }
+      add_extra_s a ev (i+j);
    }
 
 
-val aux_2s (h:words_state Blake2S) (i:nat) (input: bytes_blocks Blake2S) :
-  Lemma (requires i + 1 < pow2 32 /\ Seq.length input == i * block_length Blake2S)
+val lemma_update_s (a:hash_alg{is_blake a}) (h:words_state a) (i:nat) (input: bytes_blocks a) :
+  Lemma (requires i + 1 < pow2 32 /\ Seq.length input == i * block_length a)
         (ensures (
-          let h' = update_multi Blake2S h input in
-          v (snd h') == add_extra_s Blake2S (v (snd h)) i))
+          let h' = update_multi a h input in
+          v #U64 #SEC (snd h') == add_extra_s a (v #U64 #SEC (snd h)) i))
         (decreases i)
 
 
-val update1_add (h:words_state Blake2S) (l:bytes{Seq.length l == block_length Blake2S})
+val update1_add (a:hash_alg{is_blake a}) (h:words_state a) (l:bytes{Seq.length l == block_length a})
   : Lemma
-  (let h' = update Blake2S h l in
+  (let h' = update a h l in
    let _, ev = h in
    let _, ev' = h' in
-   ev' == add_extra_i Blake2S ev 1ul)
-let update1_add h l =
-  mul_mod_lemma (to_u64 1ul) (u64 (size_block Blake2S))
+   ev' == add_extra_i a ev 1ul)
+let update1_add a h l =
+  mul_mod_lemma (to_u64 1ul) (u64 (size_block a))
 
 #restart-solver
 #push-options "--fuel 1 --z3rlimit 20"
 
-let rec aux_2s h i input =
+let rec lemma_update_s a h i input =
   let ev = snd h in
-  let h' = update_multi Blake2S h input in
+  let h' = update_multi a h input in
   let ev' = snd h' in
-  if i = 0 then add_extra_s_zero_2s ev
+  if i = 0 then add_extra_s_zero ev
   else
-    let block, rem = split_block (block_length Blake2S) input 1 in
-    let h_mid = update Blake2S h block in
-    let h_f = update_multi Blake2S h_mid rem in
+    let block, rem = split_block (block_length a) input 1 in
+    let h_mid = update a h block in
+    let h_f = update_multi a h_mid rem in
 
     let ev_mid = snd h_mid in
     let ev_f = snd h_f in
 
     calc (==) {
-      v ev';
+      v #U64 #SEC ev';
       (==) { }
-      v ev_f;
-      (==) { aux_2s h_mid (i-1) rem }
-      add_extra_s Blake2S (v ev_mid) (i-1);
-      (==) { update1_add h block }
-      add_extra_s Blake2S (v (add_extra_i Blake2S ev 1ul)) (i-1);
+      v #U64 #SEC ev_f;
+      (==) { lemma_update_s a h_mid (i-1) rem }
+      add_extra_s a (v #U64 #SEC ev_mid) (i-1);
+      (==) { update1_add a h block }
+      add_extra_s a (v #U64 #SEC (add_extra_i a ev 1ul)) (i-1);
       (==) { calc (==) {
-        v (add_extra_i Blake2S ev 1ul);
-        (==) { add_s_i_2s ev 1ul }
-        add_extra_s Blake2S (v ev) 1;
+        v #U64 #SEC (add_extra_i a ev 1ul);
+        (==) { add_s_i a ev 1ul }
+        add_extra_s a (v #U64 #SEC ev) 1;
           }
         }
-      add_extra_s Blake2S (add_extra_s Blake2S (v ev) 1) (i-1);
-      (==) { add_extra_s_assoc_2s (v ev) (i-1) 1 }
-      add_extra_s Blake2S (v ev) i;
+      add_extra_s a (add_extra_s a (v #U64 #SEC ev) 1) (i-1);
+      (==) { add_extra_s_assoc a (v #U64 #SEC ev) (i-1) 1 }
+      add_extra_s a (v #U64 #SEC ev) i;
     }
 
 #pop-options
@@ -123,11 +115,6 @@ let rec update_multi_add_extra a h i input =
   let ev = snd h in
   let h' = update_multi a h input in
   let ev' = snd h' in
-  match a with
-  | Blake2S ->
-    add_s_i_2s ev (U32.uint_to_t i);
-    aux_2s h i input
-
-  | Blake2B -> admit()
-
+  add_s_i a ev (U32.uint_to_t i);
+  lemma_update_s a h i input
 #pop-options
